Try Stefan's definition of partial monad

src/Distributions/Coin/Model.dfy
@@ -4,10 +4,11 @@
  *******************************************************************************/
 
 module Coin.Model {
+  import Partials
   import RandomNumberGenerator
   import Monad
 
-  function Sample(s: RandomNumberGenerator.RNG): (bool, RandomNumberGenerator.RNG) {
+  function Sample(s: RandomNumberGenerator.RNG): Partials.Partial<(bool, RandomNumberGenerator.RNG)> {
     Monad.Deconstruct(s)
   }
 }
