src/Distributions/UniformPowerOfTwo/Model.dfy
@@ -5,6 +5,7 @@
 
 module UniformPowerOfTwo.Model {
   import Helper
+  import Partials
   import RandomNumberGenerator
   import Quantifier
   import Monad
@@ -36,7 +37,7 @@ module UniformPowerOfTwo.Model {
   {
     (s: RandomNumberGenerator.RNG) =>
       if n == 1 then
-        (u, s)
+        Partials.Terminating((u, s))
       else
         SampleTailRecursive(n / 2, if Monad.Head(s) then 2*u + 1 else 2*u)(Monad.Tail(s))
   }
@@ -116,26 +117,29 @@ module UniformPowerOfTwo.Model {
     ensures Monad.Bind(Sample(Helper.Power(2, m)), (u: nat) => SampleTailRecursive(Helper.Power(2, l), u))(s) == Sample(Helper.Power(2, m + l))(s)
   {
     if l == 0 {
-      calc {
-        Monad.Bind(Sample(Helper.Power(2, m)), (u: nat) => SampleTailRecursive(Helper.Power(2, l), u))(s);
-        (var (u, s') := Sample(Helper.Power(2, m))(s); SampleTailRecursive(1, u)(s'));
-        Sample(Helper.Power(2, m + l))(s);
-      }
+      match Sample(Helper.Power(2, m))(s)
+      case Diverging => {}
+      case Terminating((u, s')) =>
+        calc {
+          Monad.Bind(Sample(Helper.Power(2, m)), (u: nat) => SampleTailRecursive(Helper.Power(2, l), u))(s);
+          (SampleTailRecursive(1, u)(s'));
+          Sample(Helper.Power(2, m + l))(s);
+        }
     } else {
       assert LGreaterZero: Helper.Power(2, l) >= 1 by { Helper.PowerGreater0(2, l); }
       assert MGreaterZero: Helper.Power(2, m) >= 1 by { Helper.PowerGreater0(2, m); }
       assert L1GreaterZero: Helper.Power(2, l - 1) >= 1 by { Helper.PowerGreater0(2, l - 1); }
       calc {
         Monad.Bind(Sample(Helper.Power(2, m)), (u: nat) => SampleTailRecursive(Helper.Power(2, l), u))(s);
-        (var (u, s') := Sample(Helper.Power(2, m))(s); SampleTailRecursive(Helper.Power(2, l), u)(s'));
+        (var (u, s') :- Sample(Helper.Power(2, m))(s); SampleTailRecursive(Helper.Power(2, l), u)(s'));
         { reveal LGreaterZero; }
-        (var (u, s') := Sample(Helper.Power(2, m))(s);
+        (var (u, s') :- Sample(Helper.Power(2, m))(s);
          SampleTailRecursive(Helper.Power(2, l) / 2, if Monad.Head(s') then 2 * u + 1 else 2 * u)(Monad.Tail(s')));
         { assert Helper.Power(2, l) / 2 == Helper.Power(2, l - 1); reveal L1GreaterZero; }
-        (var (u', s') := Monad.Bind(Sample(Helper.Power(2, m)), UnifStep)(s);
+        (var (u', s') :- Monad.Bind(Sample(Helper.Power(2, m)), UnifStep)(s);
          SampleTailRecursive(Helper.Power(2, l - 1), u')(s'));
         { assert Helper.Power(2, m + 1) / 2 == Helper.Power(2, m); }
-        (var (u', s') := Sample(Helper.Power(2, m + 1))(s);
+        (var (u', s') :- Sample(Helper.Power(2, m + 1))(s);
          SampleTailRecursive(Helper.Power(2, l - 1), u')(s'));
         Monad.Bind(Sample(Helper.Power(2, m + 1)), (u: nat) => SampleTailRecursive(Helper.Power(2, l - 1), u))(s);
         { RelateWithTailRecursive(l - 1, m + 1, s); }
