src/ProbabilisticProgramming/Partials.dfy
@@ -1,0 +1,39 @@
+module Partials {
+  datatype Partial<T> = Diverging | Terminating(value: T) {
+    predicate IsFailure() {
+      Diverging?
+    }
+
+    function PropagateFailure<U>(): Partial<U> {
+      Diverging
+    }
+
+    function Extract(): T
+      requires !IsFailure()
+    {
+      this.value
+    }
+
+    function Map<U>(f: T -> U): Partial<U> {
+      match this
+      case Terminating(value) => Terminating(f(value))
+      case Diverging => Diverging
+    }
+
+    function UnwrapOr(default: T): T {
+      match this
+      case Terminating(value) => value
+      case Diverging => default
+    }
+
+    function Satisfies(f: T -> bool): bool {
+      this.Map(f).UnwrapOr(false)
+    }
+
+    function Bind<U>(f: T -> Partial<U>): Partial<U> {
+      match this
+      case Terminating(value) => f(value)
+      case Diverging => Diverging
+    }
+  }
+}
